finished major proof

keyCert.v
@@ -1,467 +1,597 @@
 
-Require Import Coq.Init.Nat.
-Require Import Coq.Lists.List.
-Import ListNotations.
+  Require Import Coq.Init.Nat.
+  Require Import Coq.Lists.List.
+  Import ListNotations.
 
 
 
-(* Keys *)
-(* **** *)
-
-Definition key_id := nat.
-
-Inductive restrict_att : Type :=
-| Restricted
-| NonRestricted.
-
-Inductive sign_att : Type :=
-| Signing
-| NonSigning.
-
-Inductive decrypt_att : Type :=
-| Decrypting
-| NonDecrypting.
 
 
-Inductive pubKey : Type :=
-| Public : key_id -> restrict_att -> sign_att -> decrypt_att -> pubKey.
-
-Inductive privKey : Type :=
-| Private : key_id -> restrict_att -> sign_att -> decrypt_att -> privKey.
+(* TPM Keys *)
+(* ******** *)
 
 
-Definition pubtoPrivKey (k : pubKey) : privKey :=
-  match k with
-  | Public i r s d => Private i r s d
+(* Each key pair has a unique identifier *)
+  Definition key_id := nat.
+
+
+(* Attributes relevant to this specification *)
+
+  Inductive restrict_att : Type :=
+  | Restricted
+  | NonRestricted.
+
+  Inductive sign_att : Type :=
+  | Signing
+  | NonSigning.
+
+  Inductive decrypt_att : Type :=
+  | Decrypting
+  | NonDecrypting.
+
+
+(* Key pair definitions *)
+
+  Inductive pubKey : Type :=
+  | Public : key_id -> restrict_att -> sign_att -> decrypt_att -> pubKey.
+
+  Inductive privKey : Type :=
+  | Private : key_id -> restrict_att -> sign_att -> decrypt_att -> privKey.
+
+
+(* Functions to get a key's inverse *)
+
+  Definition pubtoPrivKey (k : pubKey) : privKey :=
+    match k with
+    | Public i r s d => Private i r s d
+    end.
+
+  Definition privToPubKey (k : privKey) : pubKey :=
+    match k with
+    | Private i r s d => Public i r s d
+    end.
+
+
+(* Attribute requirements for EK, AK, DevID, and CA keys *)
+
+  Definition endorsementKey (k : pubKey) : Prop :=
+    match k with
+    | Public _ Restricted NonSigning Decrypting => True
+    | _ => False
+    end.
+
+  Definition attestationKey (k : pubKey) : Prop :=
+    match k with
+    | Public _ Restricted Signing NonDecrypting => True
+    | _ => False
+    end.
+
+  Definition devidKey (k : pubKey) : Prop :=
+    match k with
+    | Public _ NonRestricted Signing NonDecrypting => True
+    | _ => False
+    end.
+
+  Definition caKey (k : pubKey) : Prop :=
+    match k with
+    | Public _ NonRestricted Signing _ => True
+    | _ => False
+    end.
+
+(* Roles in this specification *)
+(* Currently unused. Should include adversary? *)
+  Inductive entity : Set :=
+  | tm
+  | oem
+  | owner.
+
+
+
+(* Commands *)
+(* ******** *)
+
+
+(* Arbitrary type to model random numbers *)
+  Definition randType := nat.
+
+(* Messages includes all structures required in this specification *)
+  Inductive message : Type :=
+  | publicKey : pubKey -> message
+  | privateKey : privKey -> message
+  | rand : randType -> message
+  | hash : message -> message
+  | sign : message -> privKey -> message
+  | TPM2B_Attest : pubKey -> message
+  | credential : message -> randType -> message
+  | encrypt : message -> pubKey -> message
+  | TCG_CSR_IDevID : message -> pubKey -> message
+  | TCG_CSR_LDevID : message -> message -> message
+  | certificate : pubKey -> message    (* TODO: pubKey -> id -> message *)
+  | pair : message -> message -> message.
+
+
+(* Includes both TPM and non-TPM commands required in this specification *)
+  Inductive command : Type :=
+  | CheckAttributes : pubKey -> restrict_att -> sign_att -> decrypt_att -> command
+  | TPM2_GetRandom : randType -> command
+  | CheckNonce : message -> randType -> command
+  | TPM2_Hash : message -> command
+  | CheckHash : message -> message -> command
+  | TPM2_Sign : message -> privKey -> command
+  | CheckSig : message -> pubKey -> command
+  | TPM2_Certify : pubKey -> privKey -> command
+  | TPM2_MakeCredential : message -> randType -> pubKey -> command
+  | TPM2_ActivateCredential : message -> privKey -> privKey -> command
+  | MakeCSR_IDevID : message -> pubKey -> command
+  | MakeCSR_LDevID : message -> message -> command
+  | MakeCert : pubKey -> privKey -> command  (* TODO: pubKey -> id -> privKey -> message *)
+  | CheckCert : message -> pubKey -> command
+  | Sequence : command -> command -> command.
+
+
+(* State corresponds to what an entity knows *)
+(* Not necessarily exhaustive *)
+  Definition state := list message.
+
+
+(* TPM State contains everything produced by a TPM command *)
+(* Subset of the general state *)
+  Definition tpm_state := list message.
+
+
+(* Notations for pairs of messages and sequences of commands *)
+  Notation "m1 ,, m2" := (pair m1 m2)  (at level 90, left associativity).
+  Notation "c1 ;; c2" := (Sequence c1 c2) (at level 90, left associativity).
+
+
+
+
+
+(* Execution of Commands *)
+(* ********************* *)
+
+
+(* Inductive proposition describing command execution *)
+  Inductive execute : tpm_state * state -> command -> tpm_state * state -> Prop :=
+(*
+  CheckAttributes
+  ***************
+  Inputs: 
+    Public Key
+    Attributes
+  Success Conditions:
+    Public Key has all Attributes
+  Updates to State:
+    None
+*)
+  | E_CheckAttributes : forall stTPM st i r s d,
+      execute (stTPM, st)
+              (CheckAttributes (Public i r s d) r s d)
+              (stTPM,
+               st)
+(*
+  TPM2_GetRandom
+  **************
+  Inputs: 
+    Random Number
+  Success Conditions:
+    None
+  Updates to State:
+    Random Number to TPM State
+*)
+  | E_GetRandom : forall stTPM st g,
+      execute 
+        (stTPM, st)
+        (TPM2_GetRandom g)
+        (rand g :: stTPM,
+         rand g :: st)
+(*
+  CheckNonce
+  **********
+  Inputs: 
+    Random Number
+    Golden Value
+  Success Conditions:
+    Golden Value resides in TPM
+    Random Number is Golden Value
+  Updates to State:
+    None
+*)
+  | E_CheckNonce : forall stTPM st g,
+      In (rand g) stTPM ->
+      execute (stTPM, st)
+              (CheckNonce (rand g) g)
+              (stTPM,
+               st)
+(*
+  TPM2_Hash
+  *********
+  Inputs: 
+    Message
+  Success Conditions:
+    None
+  Updates to State:
+    The hash of Message to TPM State
+*)
+  | E_Hash : forall stTPM st m,
+      In m st ->
+      execute (stTPM, st)
+              (TPM2_Hash m)
+              (hash m :: stTPM,
+               hash m :: st)
+(*
+  CheckHash
+  *********
+  Inputs: 
+    Hash
+    Message
+  Success Conditions:
+    Hash is in state
+    Message is in state
+    Hash is the hash of Message
+  Updates to State:
+    None
+*)
+  | E_CheckHash : forall stTPM st m,
+      In (hash m) st ->
+      In m st ->
+      execute (stTPM, st)
+              (CheckHash (hash m) m)
+              (stTPM,
+               st)
+(*
+  TPM2_Sign
+  *********
+  Inputs: 
+    Message
+    Private Key
+  Success Conditions:
+    Private Key resides in TPM
+    Message resides in TPM
+    Private Key has Restricted and Signing attributes
+  Updates to State:
+    Message signed by Private Key to TPM State
+*)
+  | E_SignR : forall stTPM st m i d,
+      In (privateKey (Private i Restricted Signing d)) stTPM ->
+      In m stTPM ->
+      execute (stTPM,st)
+              (TPM2_Sign m (Private i Restricted Signing d))
+              (sign m (Private i Restricted Signing d) :: stTPM,
+               sign m (Private i Restricted Signing d) :: st)
+(*
+  TPM2_Sign
+  *********
+  Inputs: 
+    Message
+    Private Key
+  Success Conditions:
+    Private Key resides in TPM
+    Message is in state
+    Private Key has NonRestricted and Signing attributes
+  Updates to State:
+    Message signed by Private Key to TPM State
+*)
+  | E_SignNR : forall stTPM st m i d,
+      In (privateKey (Private i NonRestricted Signing d)) stTPM ->
+      In m st ->
+      execute (stTPM, st)
+              (TPM2_Sign m (Private i NonRestricted Signing d))
+              (sign m (Private i NonRestricted Signing d) :: stTPM,
+               sign m (Private i NonRestricted Signing d) :: st)
+(*
+  CheckSig
+  ********
+  Inputs: 
+    Signature
+    Public Key
+  Success Conditions:
+    Signature is in state
+    Public Key is in state
+    Public Key is the inverse of the key that created Signature
+  Updates to State:
+    None
+*)
+  | E_CheckSig : forall stTPM st m i r s d,
+      In (sign m (Private i r s d)) st ->
+      In (publicKey (Public i r s d)) st ->
+      execute (stTPM, st)
+              (CheckSig (sign m (Private i r s d)) (Public i r s d))
+              (stTPM,
+               st)
+(*
+  TPM2_Certify
+  ************
+  Inputs: 
+    Public Key
+    Private Key
+  Success Conditions:
+    The inverse of Public Key resides in TPM
+    Private Key resides in TPM
+    Private Key has Signing attribute
+  Updates to State:
+    TPM2B_Attest structure of Public Key signed by Private Key to TPM State
+*)
+  | E_Certify : forall stTPM st i r s d i0 r0 d0,
+      In (privateKey (Private i r s d)) stTPM -> 
+      In (privateKey (Private i0 r0 Signing d0)) stTPM ->
+      execute (stTPM, st)
+              (TPM2_Certify (Public i r s d) (Private i0 r0 Signing d0))
+              (sign (TPM2B_Attest (Public i r s d)) (Private i0 r0 Signing d0) :: stTPM,
+               sign (TPM2B_Attest (Public i r s d)) (Private i0 r0 Signing d0) :: st)
+(*
+  TPM2_MakeCredential
+  *******************
+  Inputs: 
+    Message
+    Random Number
+    Public Key
+  Success Conditions:
+    Message in in state
+    Random Number resides in TPM
+    Public Key has Decrypting attribute
+  Updates to State:
+    Credential structure of Message and Random Number encrypted with Public Key to TPM State
+*)
+  | E_MakeCredential : forall stTPM st m g i r s,
+      In m st ->
+      In (rand g) stTPM ->
+      In (publicKey (Public i r s Decrypting)) st ->
+      execute (stTPM, st)
+              (TPM2_MakeCredential m g (Public i r s Decrypting)) 
+              (encrypt (credential m g) (Public i r s Decrypting) :: stTPM,
+               encrypt (credential m g) (Public i r s Decrypting) :: st)
+(*
+  TPM2_ActivateCredential
+  ***********************
+  Inputs: 
+    Encrypted Credential (Credential contains Message and Random Number)
+    Private Key A
+    Private Key B
+  Success Conditions:
+    Encrypted Credential is in state
+    Private Key A resides in TPM
+    Private Key B resides in TPM
+    Private Key A is the inverse of the key that created Encrypted Credential
+    Message is the hash of the inverse of Private Key B
+  Updates to State:
+    Random Number and Credential to TPM State
+*)
+  | E_ActivateCredential : forall stTPM st m g i r s d i0 r0 s0 d0,
+      In (encrypt (credential m g) (Public i r s d)) st ->
+      In (privateKey (Private i r s d)) stTPM ->
+      In (privateKey (Private i0 r0 s0 d0)) stTPM ->
+      execute (stTPM, m::st) (CheckHash m (publicKey (Public i0 r0 s0 d0))) (stTPM, m::st) ->
+      execute (stTPM, st)
+              (TPM2_ActivateCredential (encrypt (credential m g) (Public i r s d)) 
+                                      (Private i r s d)
+                                      (Private i0 r0 s0 d0)) 
+              (rand g :: credential m g :: stTPM,
+               rand g :: credential m g :: st)
+(*
+  MakeCSR_IDevID
+  **************
+  Inputs: 
+    Message
+    Public Key
+  Success Conditions:
+    Message is in state
+    Public Key is in state
+  Updates to State:
+    TCG_CSR_IDevID of Message and Public Key to State
+*)
+  | E_MakeCSR_IDevID : forall stTPM st m i r s d,
+      In m st ->
+      In (publicKey (Public i r s d)) st ->
+      execute (stTPM, st)
+              (MakeCSR_IDevID m (Public i r s d))
+              (stTPM,
+               TCG_CSR_IDevID m (Public i r s d) :: st)
+(*
+  MakeCSR_LDevID
+  **************
+  Inputs: 
+    Message A
+    Message B
+  Success Conditions:
+    Message A is in state
+    Message B is in state
+  Updates to State:
+    TCG_CSR_LDevID of Message A and Message B to State
+*)
+  | E_MakeCSR_LDevID : forall stTPM st m1 m2,
+      In m1 st ->
+      In m2 st ->
+      execute (stTPM, st)
+              (MakeCSR_LDevID m1 m2)
+              (stTPM,
+               TCG_CSR_LDevID m1 m2 :: st)
+(*
+  MakeCert
+  ********
+  Inputs: 
+    Public Key
+    Private Key
+  Success Conditions:
+    Public Key is in state
+    Private Key resides in TPM
+    Private Key has NonRestricted and Signing attributes
+  Updates to State:
+    Certificate of Public Key signed by Private Key to TPM State
+*)
+  | E_MakeCert : forall stTPM st i r s d i0 d0,
+      In (publicKey (Public i r s d)) st ->
+      In (privateKey (Private i0 NonRestricted Signing d0)) stTPM ->
+      execute (stTPM, st)
+              (MakeCert (Public i r s d) (Private i0 NonRestricted Signing d0))
+              (sign (certificate (Public i r s d)) (Private i0 NonRestricted Signing d0) :: stTPM,
+               sign (certificate (Public i r s d)) (Private i0 NonRestricted Signing d0) :: st)
+(*
+  CheckCert
+  *********
+  Inputs: 
+    Signature
+    Public Key
+  Success Conditions:
+    Signature is in state
+    Public Key is in state
+    Signature contains Certificate
+    Public Key is the inverse of the key that created Signature
+  Updates to State:
+    None
+*)
+  | E_CheckCert : forall stTPM st k i r s d,
+      In (sign (certificate k) (Private i r s d)) st ->
+      In (publicKey (Public i r s d)) st ->
+      execute (stTPM, st)
+              (CheckCert (sign (certificate k) (Private i r s d)) (Public i r s d))
+              (stTPM,
+              st)
+(*
+  Sequence
+  ********
+  Inputs: 
+    Command A
+    Command B
+  Success Conditions:
+    None
+  Updates to State:
+    Effects from Command A and Command B
+*)
+  | E_Sequence : forall ini mid fin c1 c2,
+      execute ini c1 mid ->
+      execute mid c2 fin ->
+      execute ini (Sequence c1 c2) fin.
+
+
+(* Execute relation is a partial function *)
+  Theorem execute_deterministic : forall ini c fin1 fin2,
+    execute ini c fin1 ->
+    execute ini c fin2 ->
+    fin1 = fin2.
+  Proof.
+    intros ini c fin1 fin2 E1 E2.
+    generalize dependent fin2.
+    induction E1; intros fin2 E2; inversion E2; subst; try reflexivity.
+    assert (mid = mid0) as EQ_mid.
+    - apply IHE1_1; assumption.
+    - apply IHE1_2; rewrite EQ_mid; assumption.
+  Qed.
+
+
+  Ltac execute_constructor :=
+    match goal with
+    | [ |- execute _ (Sequence _ _) _ ] => eapply E_Sequence
+    | [ |- execute _ _ _] => constructor
+    end.
+
+
+  Theorem sequence_split : forall ini c1 c2 fin,
+    execute ini (c1 ;; c2) fin ->
+    exists mid, (execute ini c1 mid /\ execute mid c2 fin).
+  Proof.
+    intros ini c1 c2 fin H; inversion H; subst.
+    exists mid; split; assumption.
+  Qed.
+
+  Theorem checkSig_signature : forall ini fin m k,
+    execute ini (CheckSig m k) fin ->
+    exists m', m = sign m' (pubtoPrivKey k).
+  Proof.
+    intros ini fin m k H; inversion H; subst. 
+    exists m0; simpl; reflexivity.
+  Qed.
+
+  Theorem checkCert_signature : forall ini fin m k,
+    execute ini (CheckCert m k) fin ->
+    exists k', m = sign (certificate k') (pubtoPrivKey k).
+  Proof.
+    intros ini fin m k H; inversion H; subst. 
+    exists k0; simpl; reflexivity.
+  Qed.
+
+
+
+(* Message Discovery *)
+(* ***************** *)
+
+(* An entity who knows a message can discover additional messages from it *)
+  Inductive discoverable : message -> state -> Prop :=
+  | D_publicKey : forall k,
+      discoverable (publicKey k) [publicKey k]
+  | D_privateKey : forall k,
+      discoverable (privateKey k) [privateKey k]
+  | D_rand : forall r,
+      discoverable (rand r) [rand r]
+  | D_hash : forall m,
+      discoverable (hash m) [hash m]
+  | D_sign : forall m k st,               (* contents of signature *)
+      discoverable m st ->
+      discoverable (sign m k) ((sign m k)::st)
+  | D_Attest : forall k,                  (* contents of TPM2_Attest structure *)
+      discoverable (TPM2B_Attest k) [(TPM2B_Attest k); (publicKey k)] 
+  | D_credential : forall m r,
+      discoverable (credential m r) [credential m r]
+  | D_encrypt : forall m k,
+      discoverable (encrypt m k) [encrypt m k]
+  | D_CSR_IDevID : forall m k st,         (* contents of TCG_CSR_IDevID *)
+      discoverable m st ->
+      discoverable (TCG_CSR_IDevID m k) ([(TCG_CSR_IDevID m k); (publicKey k)]++st)
+  | D_CSR_LDevID : forall m1 m2 st1 st2,  (* contents of TCG_CSR_LDevID *)
+      discoverable m1 st1 ->
+      discoverable m2 st2 ->
+      discoverable (TCG_CSR_LDevID m1 m2) ((TCG_CSR_LDevID m1 m2)::st1++st2)
+  | D_certificate : forall k,             (* contents of certificate *)
+      discoverable (certificate k) [(certificate k); (publicKey k)]
+  | D_pair : forall m1 m2 st1 st2,        (* contents of pair *)
+      discoverable m1 st1 ->
+      discoverable m2 st2 -> 
+      discoverable (pair m1 m2) ((m1,,m2)::(st1++st2)).
+
+
+(* When sending a message the recipient can discover these additional messages *)
+  Fixpoint send (m : message) : state :=
+  match m with
+    | sign m0 k => ((sign m0 k)::(send m0))
+    | TPM2B_Attest k => [(TPM2B_Attest k); (publicKey k)]
+    | TCG_CSR_IDevID m0 k => ([(TCG_CSR_IDevID m0 k); publicKey k]++(send m0))
+    | TCG_CSR_LDevID m1 m2 => ((TCG_CSR_LDevID m1 m2)::(send m1)++(send m2))
+    | certificate k => [(certificate k); (publicKey k)]
+    | pair m1 m2 => ((m1,,m2)::((send m1)++(send m2)))
+    | _ => [m]
   end.
 
-Definition privToPubKey (k : privKey) : pubKey :=
-  match k with
-  | Private i r s d => Public i r s d
-  end.
 
 
-Definition endorsementKey (k : pubKey) : Prop :=
-  match k with
-  | Public _ Restricted NonSigning Decrypting => True
-  | _ => False
-  end.
+(* Discoverable relation and Send function are equivalent *)
 
-Definition attestationKey (k : pubKey) : Prop :=
-  match k with
-  | Public _ Restricted Signing NonDecrypting => True
-  | _ => False
-  end.
-
-Definition devidKey (k : pubKey) : Prop :=
-  match k with
-  | Public _ NonRestricted Signing NonDecrypting => True
-  | _ => False
-  end.
-
-Definition caKey (k : pubKey) : Prop :=
-  match k with
-  | Public _ NonRestricted Signing _ => True
-  | _ => False
-  end.
-
-(* currently unused *)
-Inductive entity : Set :=
-| tm
-| oem
-| owner.
-
-
-
-
-(* Small-Step Semantics *)
-(* ******************** *)
-
-Definition randType := nat.
-
-Inductive message : Type :=
-| publicKey : pubKey -> message
-| privateKey : privKey -> message
-| rand : randType -> message
-| hash : message -> message
-| sign : message -> privKey -> message
-| TPM2B_Attest : pubKey -> message
-| credential : message -> randType -> message
-| encrypt : message -> pubKey -> message
-| TCG_CSR_IDevID : message -> pubKey -> message
-| TCG_CSR_LDevID : message -> message -> message
-| certificate : pubKey -> message    (* TODO: pubKey -> id -> message *)
-| pair : message -> message -> message.
-
-
-
-Inductive command : Type :=
-| CheckAttributes : pubKey -> restrict_att -> sign_att -> decrypt_att -> command
-| TPM2_GetRandom : randType -> command
-| CheckNonce : message -> randType -> command
-| TPM2_Hash : message -> command
-| CheckHash : message -> message -> command
-| TPM2_Sign : message -> privKey -> command
-| CheckSig : message -> pubKey -> command
-| TPM2_Certify : pubKey -> privKey -> command
-| TPM2_MakeCredential : message -> randType -> pubKey -> command
-| TPM2_ActivateCredential : message -> privKey -> privKey -> command
-| MakeCSR_IDevID : message -> pubKey -> command
-| MakeCSR_LDevID : message -> message -> command
-| MakeCert : pubKey -> privKey -> command  (* TODO: pubKey -> id -> privKey -> message *)
-| Sequence : command -> command -> command.
-
-(* corresponds to what an entity knows *)
-Definition state := list message. (* not necessarily exhaustive *)
-
-(* contains everything produced by a TPM command *)
-Definition tpm_state := list message. (* subset of state *)
-
-
-
-Notation "m1 ,, m2" := (pair m1 m2)  (at level 90, left associativity).
-Notation "c1 ;; c2" := (Sequence c1 c2) (at level 90, left associativity).
-
-
-Inductive execute : tpm_state * state -> command -> tpm_state * state -> Prop :=
-| E_CheckAttributes : forall stTPM st i r s d,
-    execute (stTPM, st)
-            (CheckAttributes (Public i r s d) r s d)  (* all key attributes match input *)
-            (stTPM,
-             st)
-
-| E_GetRandom : forall stTPM st g,
-    execute (stTPM, st)
-            (TPM2_GetRandom g) 
-            (rand g :: stTPM,
-             rand g :: st)
-
-| E_CheckNonce : forall stTPM st g,
-    In (rand g) stTPM ->            (* golden value secret resides in TPM *)
-    execute (stTPM, st)
-            (CheckNonce (rand g) g) (* input matches golden value *)
-            (stTPM,
-             st)
-
-| E_Hash : forall stTPM st m,
-    In m st ->                      (* message to be hashed *)
-    execute (stTPM, st)
-            (TPM2_Hash m)
-            (hash m :: stTPM,
-             hash m :: st)
-
-| E_CheckHash : forall stTPM st m,
-    In (hash m) st ->               (* hash digest *)
-    In m st ->                      (* message to check against hash *)
-    execute (stTPM, st)
-            (CheckHash (hash m) m)  (* hash of message matches digest *)
-            (stTPM,
-             st)
-
-| E_SignR : forall stTPM st m i d,                            (* must use Restricted Signing key *)
-    In (privateKey (Private i Restricted Signing d)) stTPM -> (* key resides in TPM *)
-    In m stTPM ->                                   (* message to be signed resides in same TPM *)
-    execute (stTPM,st)
-            (TPM2_Sign m (Private i Restricted Signing d))
-            (sign m (Private i Restricted Signing d) :: stTPM,
-             sign m (Private i Restricted Signing d) :: st)
-
-| E_SignNR : forall stTPM st m i d,                               (* must use NonRestricted Signing key *)
-    In (privateKey (Private i NonRestricted Signing d)) stTPM ->  (* key resides in TPM *)
-    In m st ->                                                    (* message to be signed *)
-    execute (stTPM, st)
-            (TPM2_Sign m (Private i NonRestricted Signing d))
-            (sign m (Private i NonRestricted Signing d) :: stTPM,
-             sign m (Private i NonRestricted Signing d) :: st)
-
-| E_CheckSig : forall stTPM st m i r s d,
-    In (sign m (Private i r s d)) st ->   (* signature *)
-    In (publicKey (Public i r s d)) st -> (* public part of key that performed the signature *)
-    execute (stTPM, st)
-            (CheckSig (sign m (Private i r s d)) (Public i r s d)) (* key id and attributes must be identical *)
-            (stTPM,
-             st)
-
-| E_Certify : forall stTPM st i r s d i0 r0 d0,
-    In (privateKey (Private i r s d)) stTPM ->   (* private part of key to be certified resides in TPM *)
-    In (privateKey (Private i0 r0 Signing d0)) stTPM ->  (* key to sign the TPM2_Attest structure resides in same TPM *)
-    execute (stTPM, st)
-            (TPM2_Certify (Public i r s d) (Private i0 r0 Signing d0))
-            (sign (TPM2B_Attest (Public i r s d)) (Private i0 r0 Signing d0) :: stTPM,
-             sign (TPM2B_Attest (Public i r s d)) (Private i0 r0 Signing d0) :: st)
-
-| E_MakeCredential : forall stTPM st m g i r s,
-    In m st ->                    (* hash of public part of key i.e., name of key *)
-    In (rand g) stTPM ->          (* secret resides in TPM *)
-    In (publicKey (Public i r s Decrypting)) st ->  (* key to encrypt the credential structure *)
-    execute (stTPM, st)
-            (TPM2_MakeCredential m g (Public i r s Decrypting)) 
-            (encrypt (credential m g) (Public i r s Decrypting) :: stTPM,
-             encrypt (credential m g) (Public i r s Decrypting) :: st)
-
-| E_ActivateCredential : forall stTPM st m g i r s i0 r0 s0 d0,
-    In (encrypt (credential (hash m) g) (Public i r s Decrypting)) st -> (* encrypted credential structure *)
-    In (privateKey (Private i r s Decrypting)) stTPM ->  (* key to decrypt resides in TPM *)
-    In (privateKey (Private i0 r0 s0 d0)) stTPM -> (* private part of key to be certified resides in same TPM *)
-    execute (stTPM,
-             hash m :: st)
-            (CheckHash (hash m) (publicKey (Public i0 r0 s0 d0))) (* name in credential structure matches key to be certified*)
-            (stTPM,
-             hash m :: st) ->
-    execute (stTPM, st)
-            (TPM2_ActivateCredential (encrypt (credential (hash m) g) (Public i r s Decrypting)) 
-                                     (Private i r s Decrypting)
-                                     (Private i0 r0 s0 d0)) 
-            (rand g :: credential (hash m) g :: stTPM,
-             rand g :: credential (hash m) g :: st)
-             
-| E_MakeCSR_IDevID : forall stTPM st m i r s d,
-    In m st ->                            (* EK certificate *)
-    In (publicKey (Public i r s d)) st -> (* public part of IAK *)
-    execute (stTPM, st)
-            (MakeCSR_IDevID m (Public i r s d))
-            (stTPM,
-             TCG_CSR_IDevID m (Public i r s d) :: st)
-
-| E_MakeCSR_LDevID : forall stTPM st m1 m2,
-    In m1 stTPM ->    (* signed TPM2_Attest structure resides in TPM *)
-    In m2 st ->       (* IAK certificate *)
-    execute (stTPM, st)
-            (MakeCSR_LDevID m1 m2)
-            (stTPM,
-             TCG_CSR_LDevID m1 m2 :: st)
-
-| E_MakeCert : forall stTPM st i r s d i0 d0,
-    In (publicKey (Public i r s d)) st ->                           (* key to be certified *)
-    In (privateKey (Private i0 NonRestricted Signing d0)) stTPM ->  (* key to sign the certificate resides in TPM *)
-    execute (stTPM, st)
-            (MakeCert (Public i r s d) (Private i0 NonRestricted Signing d0))
-            (sign (certificate (Public i r s d)) (Private i0 NonRestricted Signing d0) :: stTPM,
-             sign (certificate (Public i r s d)) (Private i0 NonRestricted Signing d0) :: st)
-
-| E_Sequence : forall ini mid fin c1 c2,
-    execute ini c1 mid ->
-    execute mid c2 fin ->
-    execute ini (Sequence c1 c2) fin.
-
-
-(* execute is a partial function *)
-Theorem execute_deterministic : forall ini c fin1 fin2,
-execute ini c fin1 ->
-execute ini c fin2 ->
-fin1 = fin2.
-Proof.
-  intros ini c fin1 fin2 E1 E2.
-  generalize dependent fin2.
-  induction E1; intros fin2 E2; inversion E2; subst; try reflexivity.
-  assert (mid = mid0) as EQ_mid.
-  - apply IHE1_1; assumption.
-  - apply IHE1_2; rewrite EQ_mid; assumption.
-Qed.
-
-Ltac execute_constructor :=
-match goal with
-| [ |- execute _ (Sequence _ _) _ ] => eapply E_Sequence
-| [ |- execute _ _ _] => constructor
-end.
-
-
-
-
-(* Some random theorems regarding execute *)
-
-
-Lemma sequence_first : forall ini c1 c2 fin,
-execute ini (c1 ;; c2) fin ->
-exists ini1 mid1, execute ini1 c1 mid1.
-Proof.
-  intros ini c1 c2 fin H; inversion H; subst.
-  exists ini; exists mid; assumption.
-Qed.
-
-Lemma sequence_second : forall ini c1 c2 fin,
-execute ini (c1 ;; c2) fin ->
-exists ini2 mid2, execute ini2 c2 mid2.
-Proof.
-  intros ini c1 c2 fin H; inversion H; subst.
-  exists mid; exists fin; assumption.
-Qed.
-
-Theorem sequence_split : forall ini c1 c2 fin,
-execute ini (c1 ;; c2) fin ->
-(exists ini1 mid1, execute ini1 c1 mid1) /\ 
-(exists mid2 fin2, execute mid2 c2 fin2).
-Proof.
-  intros ini c1 c2 fin H; inversion H; subst.
-  split.
-  - exists ini; exists mid; assumption.
-  - exists mid; exists fin; assumption.
-Qed.
-
-
-Print ex_intro.
-
-Lemma execute_exIntro : forall ini0 c fin0,
-execute ini0 c fin0 ->
-exists fin, execute ini0 c fin.
-Proof.
-  intros ini0 c fin0 E0;
-  eexists; apply E0.
-Qed. 
-
-
-(* failed proof *)
-Theorem ini_generalize : forall stTPM0 stTPM st0 st c fin0,
-execute (stTPM0, st0) c fin0 ->
-incl stTPM0 stTPM ->
-incl st0 st ->
-exists fin, execute (stTPM, st) c fin.
-Proof.
-  intros stTPM0 stTPM st0 st c fin0 E0 H_TPM H.
-  induction c; inversion E0; subst; eexists; execute_constructor;
-  unfold incl in *;
-    try (apply H_TPM; assumption);
-    try (apply H; assumption).
-  - inversion H9; subst; execute_constructor.
-  -- apply in_eq.
-  -- simpl in *; right; apply H; inversion H6 as [H6_left | ];
-      [inversion H6_left | assumption].
-  - (* Sequence Case *)
-
-  Restart.
-
-  intros stTPM0 stTPM st0 st c fin0 E0 H_TPM H.
-  induction c.
-  - inversion E0; subst; eexists; execute_constructor.
-  - inversion E0; subst; eexists; execute_constructor.
-  - inversion E0; subst; eexists; execute_constructor;
-    unfold incl in *;
-    try (apply H_TPM; assumption);
-    try (apply H; assumption).
-  - inversion E0; subst; eexists; execute_constructor;
-    unfold incl in *;
-    try (apply H_TPM; assumption);
-    try (apply H; assumption).
-  - inversion E0; subst; eexists; execute_constructor;
-    unfold incl in *;
-    try (apply H_TPM; assumption);
-    try (apply H; assumption).
-  - inversion E0; subst; eexists; execute_constructor;
-    unfold incl in *;
-    try (apply H_TPM; assumption);
-    try (apply H; assumption).
-  - inversion E0; subst; eexists; execute_constructor;
-    unfold incl in *;
-    try (apply H_TPM; assumption);
-    try (apply H; assumption).
-  - inversion E0; subst; eexists; execute_constructor;
-    unfold incl in *;
-    try (apply H_TPM; assumption);
-    try (apply H; assumption).
-  - inversion E0; subst; eexists; execute_constructor;
-    unfold incl in *;
-    try (apply H_TPM; assumption);
-    try (apply H; assumption).
-  - inversion E0; subst; eexists; execute_constructor;
-    unfold incl in *;
-    try (apply H_TPM; assumption);
-    try (apply H; assumption).
-    inversion H9; subst; execute_constructor.
-    -- apply in_eq.
-    -- simpl in *; right; apply H; inversion H6 as [H6_left | ];
-        [inversion H6_left | assumption].
-  - inversion E0; subst; eexists; execute_constructor;
-    unfold incl in *;
-    try (apply H_TPM; assumption);
-    try (apply H; assumption).
-  - inversion E0; subst; eexists; execute_constructor;
-    unfold incl in *;
-    try (apply H_TPM; assumption);
-    try (apply H; assumption).
-  - inversion E0; subst; eexists; execute_constructor;
-    unfold incl in *;
-    try (apply H_TPM; assumption);
-    try (apply H; assumption).
-  - (* Sequence Case *)
-Abort.
-
-
-(* Discovery *)
-(* ********* *)
-
-(* an entity who knows a message can discover additional messages from it *)
-Inductive discoverable : message -> state -> Prop :=
-| D_publicKey : forall k,
-    discoverable (publicKey k) [publicKey k]
-| D_privateKey : forall k,
-    discoverable (privateKey k) [privateKey k]
-| D_rand : forall r,
-    discoverable (rand r) [rand r]
-| D_hash : forall m,
-    discoverable (hash m) [hash m]
-| D_sign : forall m k st,               (* contents of signature *)
+  Lemma discoverableSend : forall m st,
     discoverable m st ->
-    discoverable (sign m k) ((sign m k)::st)
-| D_Attest : forall k,                  (* contents of TPM2_Attest structure *)
-    discoverable (TPM2B_Attest k) [(TPM2B_Attest k); (publicKey k)] 
-| D_credential : forall m r,
-    discoverable (credential m r) [credential m r]
-| D_encrypt : forall m k,
-    discoverable (encrypt m k) [encrypt m k]
-| D_CSR_IDevID : forall m k st,  (* contents of TCG_CSR_IDevID *)
-    discoverable m st ->
-    discoverable (TCG_CSR_IDevID m k) ([(TCG_CSR_IDevID m k); (publicKey k)]++st)
-| D_CSR_LDevID : forall m1 m2 st1 st2,  (* contents of TCG_CSR_LDevID *)
-    discoverable m1 st1 ->
-    discoverable m2 st2 ->
-    discoverable (TCG_CSR_LDevID m1 m2) ((TCG_CSR_LDevID m1 m2)::st1++st2)
-| D_certificate : forall k,             (* contents of certificate *)
-    discoverable (certificate k) [(certificate k); (publicKey k)]
-| D_pair : forall m1 m2 st1 st2,        (* contents of pair *)
-    discoverable m1 st1 ->
-    discoverable m2 st2 -> 
-    discoverable (pair m1 m2) ((m1,,m2)::(st1++st2)).
+    send m = st.
+  Proof.
+    intros m st H; induction H; simpl; subst; reflexivity.
+  Qed.
 
+  Lemma sendDiscoverable' : forall m,
+    discoverable m (send m).
+  Proof.
+    intros m; induction m; simpl; constructor; assumption.
+  Qed.
 
-(* when sending a message the recipient can discover these additional messages *)
-Fixpoint send (m : message) : state :=
-match m with
-  | sign m0 k => ((sign m0 k)::(send m0))
-  | TPM2B_Attest k => [(TPM2B_Attest k); (publicKey k)]
-  | TCG_CSR_IDevID m0 k => ([(TCG_CSR_IDevID m0 k); publicKey k]++(send m0))
-  | TCG_CSR_LDevID m1 m2 => ((TCG_CSR_LDevID m1 m2)::(send m1)++(send m2))
-  | certificate k => [(certificate k); (publicKey k)]
-  | pair m1 m2 => ((m1,,m2)::((send m1)++(send m2)))
-  | _ => [m]
-end.
-    
-Lemma discoverableSend : forall m st,
-discoverable m st ->
-send m = st.
-Proof.
-  intros m st H; induction H; simpl; subst; reflexivity.
-Qed.
+  Lemma sendDiscoverable : forall m st,
+    send m = st -> 
+    discoverable m st.
+  Proof.
+    intros m st H; induction m; subst; apply sendDiscoverable'.
+  Qed.
 
-Lemma sendDiscoverable' : forall m,
-discoverable m (send m).
-Proof.
-  intros m; induction m; simpl; constructor; assumption.
-Qed.
-
-Lemma sendDiscoverable : forall m st,
-send m = st -> 
-discoverable m st.
-Proof.
-  intros m st H; induction m; subst; apply sendDiscoverable'.
-Qed.
-
-Theorem iff_DiscoverableSend : forall m st,
-discoverable m st <-> send m = st.
-Proof.
-  split.
-  - apply discoverableSend.
-  - apply sendDiscoverable.
-Qed.
+  Theorem iff_DiscoverableSend : forall m st,
+    discoverable m st <-> send m = st.
+  Proof.
+    split.
+    - apply discoverableSend.
+    - apply sendDiscoverable.
+  Qed.
 
 
 
@@ -485,131 +615,130 @@ Qed.
 Module Type IAK_Cert_Protocol.
 
 (* OEM parameters *)
-Parameter pubNewKey : pubKey.
-Parameter privNewKey : privKey.
-Parameter pubEK : pubKey.
-Parameter privEK : privKey.
-Parameter certEK : message.
+  Parameter pubNewKey : pubKey.
+  Parameter privNewKey : privKey.
+  Parameter pubEK : pubKey.
+  Parameter privEK : privKey.
+  Parameter certEK : message.
 
 (* CA parameters *)
-Parameter pubCA : pubKey.
-Parameter privCA : privKey.
-Parameter pubTM : pubKey.
-Parameter r : randType.
+  Parameter pubCA : pubKey.
+  Parameter privCA : privKey.
+  Parameter pubTM : pubKey.
+  Parameter r : randType.
 
 
 
-Definition iniTPM : tpm_state :=
-[ publicKey pubNewKey ; (* IAK public *)
-  privateKey privNewKey ;   (* IAK private *)
-  publicKey pubEK ;         (* EK public *)
-  privateKey privEK ].           (* EK private *)
+  Definition iniTPM : tpm_state :=
+  [ publicKey pubNewKey ;
+    privateKey privNewKey ;
+    publicKey pubEK ;
+    privateKey privEK ].
 
-Definition ini : state :=
-[ publicKey pubNewKey ;
-  privateKey privNewKey ;
-  certEK ;    (* EK certificate *)
-  publicKey pubEK ;
-  privateKey privEK ].
-
-
-Definition c1 : command :=
-MakeCSR_IDevID certEK pubNewKey ;; (* 1 *)
-TPM2_Hash (TCG_CSR_IDevID certEK pubNewKey) ;;     (* 2 *)
-TPM2_Sign (hash (TCG_CSR_IDevID certEK pubNewKey)) privNewKey.                  (* 3 *)
+  Definition ini : state :=
+  [ publicKey pubNewKey ;
+    privateKey privNewKey ;
+    certEK ;    (* EK certificate *)
+    publicKey pubEK ;
+    privateKey privEK ].
 
 
-Definition midTPM : state :=
-sign (hash (TCG_CSR_IDevID certEK pubNewKey)) privNewKey :: (* 3 *)
-hash (TCG_CSR_IDevID certEK pubNewKey) ::                               (* 2 *)
-iniTPM.
-
-Definition mid : state :=
-sign (hash (TCG_CSR_IDevID certEK pubNewKey)) privNewKey :: (* 3 *)
-hash (TCG_CSR_IDevID certEK pubNewKey) ::                               (* 2 *)
-(TCG_CSR_IDevID certEK pubNewKey) ::                                    (* 1 *)
-ini.
+  Definition c1 : command :=
+  MakeCSR_IDevID certEK pubNewKey ;;                              (* 1 *)
+  TPM2_Hash (TCG_CSR_IDevID certEK pubNewKey) ;;                  (* 2 *)
+  TPM2_Sign (hash (TCG_CSR_IDevID certEK pubNewKey)) privNewKey.  (* 3 *)
 
 
-(*
-send ((TCG_CSR_IDevID certEK pubNewKey),, (sign (hash (TCG_CSR_IDevID certEK pubNewKey)) privNewKey))   (* 4 *)
-*)
+  Definition midTPM : state :=
+  sign (hash (TCG_CSR_IDevID certEK pubNewKey)) privNewKey ::
+  hash (TCG_CSR_IDevID certEK pubNewKey) ::
+  iniTPM.
 
-Definition iniTPM_CA : tpm_state :=
-[ privateKey privCA ;   (* OEM CA private *)
-  publicKey pubCA ]. (* OEM CA public *)
-
-Definition ini_CA : state :=
-[ publicKey pubTM ;    (* TM CA public*)
-  privateKey privCA ;
-  publicKey pubCA ].
-
-
-Definition c1_CA : command :=
-CheckHash (hash (TCG_CSR_IDevID certEK pubNewKey)) (TCG_CSR_IDevID certEK pubNewKey) ;;     (* 5a *)
-CheckSig (sign (hash (TCG_CSR_IDevID certEK pubNewKey)) privNewKey) pubNewKey ;;           (* 5b *)
-CheckSig certEK pubTM ;;           (* 5c *)
-CheckAttributes pubNewKey Restricted Signing NonDecrypting ;;                    (* 5d *)
-TPM2_Hash (publicKey pubNewKey) ;;                              (* 6 *)
-TPM2_GetRandom r ;;                                                   (* 7 *)
-TPM2_MakeCredential (hash (publicKey pubNewKey)) r pubEK. (* 8 *)
-
-
-Definition midTPM_CA : tpm_state :=
-encrypt (credential (hash (publicKey pubNewKey)) r) pubEK ::  (* 8 *)
-rand r ::                                                                 (* 7 *)
-hash (publicKey pubNewKey) ::                                       (* 6 *)
-iniTPM_CA.
-
-Definition mid_CA : state :=
-encrypt (credential (hash (publicKey pubNewKey)) r) pubEK ::  (* 8 *)
-rand r ::                                                                 (* 7 *)
-hash (publicKey pubNewKey) ::                                       (* 6 *)
-send ((TCG_CSR_IDevID certEK pubNewKey),, (sign (hash (TCG_CSR_IDevID certEK pubNewKey)) privNewKey)) ++ (* 4 *)
-ini_CA.
-
+  Definition mid : state :=
+  sign (hash (TCG_CSR_IDevID certEK pubNewKey)) privNewKey ::
+  hash (TCG_CSR_IDevID certEK pubNewKey) ::
+  (TCG_CSR_IDevID certEK pubNewKey) ::
+  ini.
 
 (*
-send (encrypt (credential (hash (publicKey pubNewKey)) r) pubEK)   (* 9 *)
+  send ((TCG_CSR_IDevID certEK pubNewKey),, (sign (hash (TCG_CSR_IDevID certEK pubNewKey)) privNewKey))   (* 4 *)
 *)
 
-Definition c2 : command :=
-TPM2_ActivateCredential (encrypt (credential (hash (publicKey pubNewKey)) r) pubEK) privEK (privNewKey).  (* 10 *)
-                        
 
-Definition finTPM : tpm_state :=
-rand r ::                                            (* 10 *)
-credential (hash (publicKey pubNewKey)) r ::   (* 10 *)
-midTPM.
+  Definition iniTPM_CA : tpm_state :=
+  [ privateKey privCA ;
+    publicKey pubCA ].
 
-Definition fin : state :=
-rand r ::                                                                        (* 10 *)
-credential (hash (publicKey pubNewKey)) r  ::                               (* 10 *)
-send (encrypt (credential (hash (publicKey pubNewKey)) r) pubEK) ++  (* 9 *)
-mid.
+  Definition ini_CA : state :=
+  [ publicKey pubTM ;
+    privateKey privCA ;
+    publicKey pubCA ].
+
+
+  Definition c1_CA : command :=
+  CheckHash (hash (TCG_CSR_IDevID certEK pubNewKey)) (TCG_CSR_IDevID certEK pubNewKey) ;; (* 5a *)
+  CheckSig (sign (hash (TCG_CSR_IDevID certEK pubNewKey)) privNewKey) pubNewKey ;;        (* 5b *)
+  CheckCert certEK pubTM ;;                                                               (* 5c *)
+  CheckAttributes pubNewKey Restricted Signing NonDecrypting ;;                           (* 5d *)
+  TPM2_Hash (publicKey pubNewKey) ;;                                                      (* 6 *)
+  TPM2_GetRandom r ;;                                                                     (* 7 *)
+  TPM2_MakeCredential (hash (publicKey pubNewKey)) r pubEK.                               (* 8 *)
+
+
+  Definition midTPM_CA : tpm_state :=
+  encrypt (credential (hash (publicKey pubNewKey)) r) pubEK ::
+  rand r ::
+  hash (publicKey pubNewKey) ::
+  iniTPM_CA.
+
+  Definition mid_CA : state :=
+  encrypt (credential (hash (publicKey pubNewKey)) r) pubEK ::
+  rand r ::
+  hash (publicKey pubNewKey) ::
+  send ((TCG_CSR_IDevID certEK pubNewKey),, (sign (hash (TCG_CSR_IDevID certEK pubNewKey)) privNewKey)) ++
+  ini_CA.
 
 (*
-send (rand r)    (* 11 *)
+  send (encrypt (credential (hash (publicKey pubNewKey)) r) pubEK)    (* 9 *)
 *)
 
-Definition c2_CA : command :=
-CheckNonce (rand r) r ;;                           (* 12 *)
-MakeCert pubNewKey privCA.  (* 13 *)
+  Definition c2 : command :=
+  TPM2_ActivateCredential (encrypt (credential (hash (publicKey pubNewKey)) r) pubEK) privEK (privNewKey).  (* 10 *)
 
-Definition finTPM_CA : state := 
-sign (certificate pubNewKey) privCA ::  (* 13 *)
-midTPM_CA.
 
-Definition fin_CA : state := 
-sign (certificate pubNewKey) privCA ::  (* 13 *)
-send (rand r) ++                                               (* 11 *)
-mid_CA.
+  Definition finTPM : tpm_state :=
+  rand r ::
+  credential (hash (publicKey pubNewKey)) r ::
+  midTPM.
+
+  Definition fin : state :=
+  rand r ::
+  credential (hash (publicKey pubNewKey)) r  ::
+  send (encrypt (credential (hash (publicKey pubNewKey)) r) pubEK) ++
+  mid.
+
+(*
+  send (rand r)    (* 11 *)
+*)
+
+  Definition c2_CA : command :=
+  CheckNonce (rand r) r ;;    (* 12 *)
+  MakeCert pubNewKey privCA.  (* 13 *)
+
+  Definition finTPM_CA : state := 
+  sign (certificate pubNewKey) privCA ::
+  midTPM_CA.
+
+  Definition fin_CA : state := 
+  sign (certificate pubNewKey) privCA ::
+  send (rand r) ++
+  mid_CA.
 
 
 (* Line A in 'Relationships of Keys/Certificates' diagram *)
 Axiom CertIAK_spec :
 execute (iniTPM, ini) c1 (midTPM, mid) /\     (* Steps 0 - 3 *)
-In (TCG_CSR_IDevID certEK pubNewKey) mid /\ (* Step 4 *)
+In (TCG_CSR_IDevID certEK pubNewKey) mid /\   (* Step 4 *)
 In (sign (hash (TCG_CSR_IDevID certEK pubNewKey)) privNewKey) mid /\  (* Step 4 *)
 execute (iniTPM_CA, send ((TCG_CSR_IDevID certEK pubNewKey),, sign (hash (TCG_CSR_IDevID certEK pubNewKey)) privNewKey) ++ ini_CA)
          c1_CA                                (* Steps 5 - 8*)
@@ -624,31 +753,81 @@ execute (midTPM_CA, send (rand r) ++ mid_CA)
         (finTPM_CA, fin_CA).
 
 
+Axiom unique_keys :
+pubTM = pubEK -> False.
 
-
+Axiom unique_keys' :
+pubCA = pubEK -> False.
 
 (* Protocol Assurances *)
 (* ******************* *)
 
-(* all failed proofs (need additional helper lemmas) *)
 
 (* A TPM is authentic *)
-(* [EK Certificate is valid] *)
-Theorem authenticTPM : exists success,
-execute (iniTPM_CA, certEK :: ini_CA)
-        (CheckSig certEK pubTM)
-         success.
-Proof.
-Abort.
+(* EK Certificate is valid *)
+  Theorem authenticTPM : exists st st',
+    execute st (CheckCert certEK pubTM) st'.
+  Proof.
+    assert (H : execute (iniTPM_CA, send ((TCG_CSR_IDevID certEK pubNewKey),, sign (hash (TCG_CSR_IDevID certEK pubNewKey)) privNewKey) ++ ini_CA) c1_CA (midTPM_CA, mid_CA)).
+    - apply CertIAK_spec.
+    - repeat (apply sequence_split in H; destruct H; destruct H).
+      eexists; eexists; apply H4.
+  Qed.
+
 
 (* This specific TPM is authentic and is represented by the EK Certificate *)
-(* [EK resident in this TPM corresponds to the EK Certificate] *)
-(* Theorem authenticThisTPM *)
+(* EK resident in this TPM corresponds to the EK Certificate *)
+  Theorem authenticThisTPM : 
+    certEK = sign (certificate pubEK) (pubtoPrivKey pubTM).
+  Proof.
+    assert (H_CheckCert : exists st st', execute st (CheckCert certEK pubTM) st').
+    - apply authenticTPM.
+    - destruct H_CheckCert as [ini H_CheckCert]. destruct H_CheckCert as [fin H_CheckCert].
+      inversion H_CheckCert. subst. simpl.
+      assert (H_H : execute (iniTPM_CA, send ((TCG_CSR_IDevID certEK pubNewKey),, sign (hash (TCG_CSR_IDevID certEK pubNewKey)) privNewKey) ++ ini_CA) c1_CA (midTPM_CA, mid_CA)).
+      -- apply CertIAK_spec.
+      -- unfold c1_CA in H_H. apply sequence_split in H_H. destruct H_H. destruct H1. repeat (apply sequence_split in H1; destruct H1; destruct H1).
+          inversion H3. subst. simpl in H20.
+          destruct H20 as [H20|H20]. inversion H20.
+          destruct H20 as [H20|H20]. inversion H20.
+          destruct H20 as [H20|H20]. inversion H20.
+          destruct H20 as [H20|H20]. inversion H20.
+          destruct H20 as [H20|H20].
+          inversion H7. subst. rewrite <- H13 in H20. inversion H20.
+          rewrite <- H in H20. unfold ini_CA in H20. simpl in H20.
+          destruct H20 as [H20|H20]. inversion H20.
+          destruct H20 as [H20|H20]. inversion H20.
+          destruct H20 as [H20|H20]. inversion H20. reflexivity.
+          destruct H20 as [H20|H20]. inversion H20.
+          destruct H20 as [H20|H20]. inversion H20.
+          destruct H20 as [H20|H20]. inversion H20. rewrite H12 in H11. apply unique_keys in H11. inversion H11.
+          destruct H20 as [H20|H20]. inversion H20.
+          destruct H20 as [H20|H20]. inversion H20. rewrite H12 in H11. apply unique_keys' in H11. inversion H11.
+          inversion H20.
+  Qed.
+          
+          
+  Abort.
 
-  
+  Theorem test: forall m,
+  certEK = m -> 
+  False.
+Proof.
+  intros m H. induction m.
+Abort.
+
+
+
 (* This AK is authentic *)
-(* [AK in CSR is resident in the same TPM as the EK] *)
-(* authenticAK *)
+(* AK in CSR is resident in the same TPM as the EK *)
+  Theorem authenticThisAK :
+    In (privateKey privNewKey) finTPM /\
+    In (privateKey privEK) finTPM.
+  Proof.
+    unfold finTPM; unfold midTPM; unfold iniTPM;
+    split; simpl; auto 9.
+  Qed.
+
 
 End IAK_Cert_Protocol.
 
